Incorporated back some lemmas from later hierarchy from a different branch. Also strengthened slightly one of the axioms.

utils/Library_extra/Monoid_extra.thy
@@ -253,45 +253,55 @@ instance nat :: trace
   apply linarith+
   done
     
-subsection {* Trace algebra based on left-cancellative unitary semigroup whose
-  unitary function is idempotent. *}
-  
-text {* We call the unitary function fzero (as in a functional zero
-        when compared to the monoid-based trace algebra). *}
+text \<open> In this theory we present a variant of the trace algebra where instead of
+       a partial order we have a preorder. This is possible by generalising the
+       zero of the monoid-based trace algebra and dropping anti-symmetry.
+       Effectively we have a left-cancellative unary semigroup whose unary
+       function @{term f\<^sub>0} is idempotent.  \<close>
+
+subsection \<open> Unary fzero \<close>
+
+text \<open> We call the unitary function fzero @{term f\<^sub>0}, that is, a functional zero
+       when compared to the monoid-based trace algebra. \<close>
   
 class fzero = 
-  fixes fzero :: "'a \<Rightarrow> 'a"
-    
-class semigroup_add_fzero = semigroup_add + fzero
+  fixes fzero :: "'a \<Rightarrow> 'a" ("f0'(_')")
 
 class fzero_idem = fzero +
-  assumes fzero_idem[simp]: "fzero (fzero a) = fzero a"    
-    
-text {* The class of the monoid-based trace algebra can be obtained
-        by fixing fzero as 0. *}     
+  assumes fzero_idem[simp]: "f0(f0(a)) = f0(a)"    
+
+text \<open> The monoid-based trace algebra can be obtained by fixing @{term f\<^sub>0} as 0.
+       We explore this in the trace algebra hierarchy theory file \<close>
     
 class fzero_is_0 = fzero + zero +
-  assumes fzero_is_0: "fzero a = 0"
+  assumes fzero_is_0: "f0(a) = 0"
 
-text {* Another algebra is likely obtained by considering the identity
-        function. *}
+text \<open> If we admit @{term f\<^sub>0} to be the identity, then we obtain a semigroup that
+       belongs to the class of U-semigroups. In particular, when combined with the
+       trace algebra presented in this theory, we obtain a *-semigroup. \<close>
 
 class fzero_ident = fzero +
-  assumes fzero_ident: "fzero a = a"
+  assumes fzero_ident: "f0(a) = a"
+
+subsection \<open> Unary fzero semigroup \<close>
+
+text \<open> The class of semigroups with a unary function is then defined. \<close>
+
+class semigroup_add_fzero = semigroup_add + fzero
     
-text {* We then define mirror properties of a monoid, but instead we
-        require the zero property on fzero, rather than 0. *}    
+text \<open> We then define mirror properties of a monoid, but instead we
+       require the zero property on fzero, rather than 0. \<close>
     
 class fzero_add_zero = fzero_idem + semigroup_add_fzero +
-  assumes add_fzero_left[simp]: "(fzero a) + a = a"
-  assumes add_fzero_right[simp]: "a + (fzero a) = a"
+  assumes add_fzero_left[simp]: "f0(b) + a = a"
+  assumes add_fzero_right[simp]: "a + f0(a) = a"
     
-text {* In this algebra we only require zero_sum_right, but not
+text \<open> In this algebra we only require zero_sum_right, but not
         zero_sum_left. The immediate consequence is that we do
-        not obtain an order as there is no anti-symmetry. *}
+        not obtain an order as there is no anti-symmetry. \<close>
     
 class fzero_sum_zero = fzero_add_zero +
-  assumes fzero_sum_right: "a + b = (fzero b) \<Longrightarrow> (b = fzero b)"
+  assumes fzero_sum_right: "a + b = f0(b) \<Longrightarrow> b = f0(b)"
     
 instance fzero_sum_zero \<subseteq> fzero_add_zero
   by intro_classes  
@@ -302,109 +312,134 @@ instance fzero_add_zero \<subseteq> semigroup_add_fzero
 instance fzero_sum_zero \<subseteq> semigroup_add_fzero
   by intro_classes    
     
-text {* However, when we restrict the class to fzero_is_0, then
-        trivially we have that sum_left and sum properties are
-        satisfied as expected. *}    
+text \<open> However, when in addition we consider the class fzero_is_0, then trivially we have that 
+       sum_left and sum properties are satisfied as expected. \<close>
     
 lemma fzero_sum_left:
   fixes a :: "'a::{fzero_is_0,fzero_sum_zero}"
-  shows "a + b = fzero a \<Longrightarrow> a = fzero a"
+  shows "a + b = f0(a) \<Longrightarrow> a = f0(a)"
   by (metis fzero_add_zero_class.add_fzero_right fzero_sum_right fzero_is_0)
     
 lemma fzero_sum:
   fixes a :: "'a::{fzero_is_0,fzero_sum_zero}"
-  shows "a + b = fzero a \<longleftrightarrow> a = fzero a \<and> b = fzero b"
+  shows "a + b = f0(a) \<longleftrightarrow> a = f0(a) \<and> b = f0(b)"
   by (metis add_fzero_left fzero_is_0 fzero_sum_left)    
-    
-class fzero_is_0_sum_zero = fzero_is_0 + fzero_sum_zero
 
-instance fzero_is_0_sum_zero \<subseteq> monoid_sum_0
-  apply intro_classes
-  apply (metis add_fzero_left fzero_is_0)
-  apply (metis add_fzero_right fzero_is_0)
-  by (metis fzero_is_0 fzero_sum)
-  
-text {* We also define the less operator and minus in terms of
-        plus. *}
-    
-context semigroup_add
-begin
-  
-definition fzero_le (infix "\<le>\<^sub>d" 50)
-  where "a \<le>\<^sub>d b \<longleftrightarrow> (\<exists>c. b = a + c)"
-    
-lemma monoid_le_trans: 
-  "\<lbrakk> a \<le>\<^sub>d b; b \<le>\<^sub>d c \<rbrakk> \<Longrightarrow> a \<le>\<^sub>d c"
-  using add_assoc local.fzero_le_def by auto
-    
-lemma monoid_le_add: "a \<le>\<^sub>d a + b"
-  by (auto simp add: fzero_le_def)
+text \<open> We define less and minus in terms of plus in the context of the class fzero_add_zero
+       as this is sufficient to define a prefix relation that is reflexive and transitive. \<close>
 
-lemma monoid_le_add_left_mono: 
-  "a \<le>\<^sub>d b \<Longrightarrow> c + a \<le>\<^sub>d c + b"
-  using add_assoc local.fzero_le_def by auto
-    
-end
-  
-context semigroup_add
-begin
- 
-definition fzero_subtract (infixl "-\<^sub>d" 65)
-  where "a -\<^sub>d b = (if (b \<le>\<^sub>d a) then THE c. a = b + c else SOME c. \<forall>d. c \<le>\<^sub>d d)"  
-end                                                   (* \<forall>d. \<exists>b. d = c + b*)
- 
-text {* The class for left cancellative semigroups. *}  
-  
-class semigroup_add_left_cancel = semigroup_add + left_cancel_semigroup  
+context fzero_add_zero
 begin
   
-lemma add_monoid_diff_cancel_left [simp]: 
-  "(a + b) -\<^sub>d a = b"
-  apply (simp add: fzero_subtract_def monoid_le_add)
-  apply (rule the_equality)
-  apply (simp)
-  by (metis local.add_left_imp_eq)
+definition fzero_le (infix "\<le>us" 50)
+  where "a \<le>us b \<longleftrightarrow> (\<exists>c. b = a + c)"
+
+definition fzero_subtract (infixl "-us" 65)
+  where "a -us b = (if (b \<le>us a) then THE c. a = b + c else f0(a))"  
     
-lemma add_le_imp_le_left: 
-  "c + a \<le>\<^sub>d c + b \<Longrightarrow> a \<le>\<^sub>d b"
-  by (auto simp add:fzero_le_def, metis add_assoc local.add_monoid_diff_cancel_left)
- 
+lemma fzero_refl:
+  "a \<le>us a"
+  by (metis fzero_le_def local.add_fzero_right)
+    
+lemma fzero_le_trans: 
+  "\<lbrakk> a \<le>us b; b \<le>us c \<rbrakk> \<Longrightarrow> a \<le>us c"
+  unfolding fzero_le_def
+  using add_assoc by blast
+
+lemma fzero_le_least_fzero: "fzero a \<le>us a"
+  by (metis local.add_fzero_left local.fzero_le_def)
+   
+lemma fzero_le_add: "a \<le>us a + b"
+  using fzero_le_def
+  by blast
+
+lemma fzero_le_add_left_mono: 
+  "a \<le>us b \<Longrightarrow> c + a \<le>us c + b"
+  using fzero_le_def
+  using add_assoc by auto
+
 end
-  
-text {* This allows relating minus and ord from an existing type with
-        just the left-cancellative semigroup properties, without instantiating
-        an fzero function. *}  
-  
-class semigroup_add_left_cancel_minus_ord = semigroup_add_left_cancel + ord + minus +
- assumes le_is_fzero_le: "a \<le> b \<longleftrightarrow> (a \<le>\<^sub>d b)"
+
+text \<open> The following class allows @term{\<le>}, @term{<} and @term{-} to be related with
+       that of fzero_add_zero. \<close>
+
+class fzero_add_fzero_ord = fzero_add_zero + ord + 
+  assumes le_is_fzero_le: "a \<le> b \<longleftrightarrow> (a \<le>us b)"
   and less_iff: "a < b \<longleftrightarrow> a \<le> b \<and> \<not> (b \<le> a)"
-  and minus_def: "a - b = a -\<^sub>d b"
+  
+class fzero_add_fzero_ord_minus = fzero_add_fzero_ord + ord + minus +
+  assumes minus_def: "a - b = a -us b"
+
+text \<open> We then show we have a preorder. \<close>
+
+instance fzero_add_fzero_ord \<subseteq> preorder
+proof
+  fix x y z :: "'a::fzero_add_fzero_ord" 
+  show "(x < y) = (x \<le> y \<and> \<not> y \<le> x)"
+    by (simp add: less_iff)
+  show "x \<le> x"
+    by (simp add: fzero_add_zero_class.fzero_refl le_is_fzero_le)
+  show "x \<le> y \<Longrightarrow> y \<le> z \<Longrightarrow> x \<le> z"
+    using le_is_fzero_le 
+    by (metis fzero_add_zero_class.fzero_le_trans)
+qed
+
+subsection \<open> Unary left-cancellative fzero semigroup class \<close>
+  
+class semigroup_add_left_cancel = semigroup_add +
+  assumes add_left_imp_eq: "a + b = a + c \<Longrightarrow> b = c"
+
+class fzero_add_left_cancel = semigroup_add_left_cancel + fzero_add_zero 
+begin
+  
+lemma add_fzero_diff_cancel_left [simp]: 
+  "(a + b) -us a = b"
+  apply (simp add: fzero_subtract_def fzero_le_add)
+  apply (rule the_equality)
+   apply (simp)
+    using local.add_left_imp_eq by blast
+    
+lemma add_le_imp_le_left:
+  "c + a \<le>us c + b \<Longrightarrow> a \<le>us b"
+  unfolding fzero_le_def
+  by (metis add_assoc local.add_left_imp_eq)
+
+lemma diff_add_cancel_left': "a \<le>us b \<Longrightarrow> a + (b -us a) = b"
+  using local.fzero_subtract_def
+  by (metis add_fzero_diff_cancel_left local.fzero_le_def)
+
+lemma "b \<le>us a \<Longrightarrow> x = a -us b \<longleftrightarrow> b + x = a"
+  by (metis diff_add_cancel_left' local.add_left_imp_eq)
+
+end 
+  
+class semigroup_add_left_cancel_minus_ord = fzero_add_fzero_ord_minus + fzero_add_left_cancel
 begin
   
   lemma le_iff_add: "a \<le> b \<longleftrightarrow> (\<exists> c. b = a + c)"
     by (simp add: local.fzero_le_def local.le_is_fzero_le)
   
   lemma le_add [simp]: "a \<le> a + b"
-    using local.le_iff_add by blast
+    by (simp add: local.le_is_fzero_le local.fzero_le_add)
       
   lemma add_diff_cancel_left [simp]: "(a + b) - a = b"
     by (simp add: minus_def)
       
   lemma add_left_mono: "a \<le> b \<Longrightarrow> c + a \<le> c + b"
-    by (simp add: local.le_is_fzero_le local.monoid_le_add_left_mono)
+    by (simp add: local.le_is_fzero_le local.fzero_le_add_left_mono)
 
   lemma add_le_imp_le_left: "c + a \<le> c + b \<Longrightarrow> a \<le> b"
-    by (auto simp add: le_iff_add, metis add_assoc local.add_diff_cancel_left)
+    using local.add_le_imp_le_left local.le_is_fzero_le by blast
       
-  lemma add_diff_cancel_left' [simp]:  "(c + a) - (c + b) = a - b"
-  proof (cases "b \<le> a")
-    case True thus ?thesis
-      by (metis add_assoc local.add_diff_cancel_left local.le_iff_add)
-  next
-    case False thus ?thesis
-      using local.add_le_imp_le_left  
-      by (metis local.fzero_subtract_def local.le_is_fzero_le local.minus_def)
-  qed
+  lemma add_diff_cancel_left' [simp]:  " (c + a) - (c + b) = a - b"
+    proof (cases "b \<le> a")
+      case True thus ?thesis
+        by (metis add_assoc local.add_fzero_diff_cancel_left local.le_iff_add local.minus_def)
+    next
+      case False thus ?thesis
+        using local.add_le_imp_le_left
+        by (metis add_assoc local.add_fzero_diff_cancel_left local.add_fzero_right local.fzero_subtract_def local.le_is_fzero_le local.minus_def)
+    qed
     
   lemma diff_add_cancel_left': "a \<le> b \<Longrightarrow> a + (b - a) = b"
     using local.le_iff_add local.le_is_fzero_le by auto
@@ -413,44 +448,89 @@ begin
     using local.add_le_imp_le_left local.add_left_mono local.less_iff by blast
       
   lemma sum_minus_left: "c \<le> a \<Longrightarrow> (a + b) - c = (a - c) + b"
-    by (metis add_assoc diff_add_cancel_left' local.add_monoid_diff_cancel_left local.minus_def)      
-    
+    by (metis add_assoc diff_add_cancel_left' local.add_fzero_diff_cancel_left local.minus_def)
+  
   lemma minus_cancel_le: "\<lbrakk> x \<le> y; y \<le> z \<rbrakk> \<Longrightarrow> y - x \<le> z - x"
-    using add_assoc le_iff_add by auto
+    by (metis local.diff_add_cancel_left' local.le_is_fzero_le local.fzero_le_add local.sum_minus_left)
 
   lemma sum_minus_right: "c \<ge> a \<Longrightarrow> a + b - c = b - (c - a)"
     by (metis diff_add_cancel_left' local.add_diff_cancel_left') 
   
   lemma diff_diff_add: "b + c \<le> a \<Longrightarrow> a - (b + c) = a - b - c"
-    by (metis local.add_diff_cancel_left local.diff_add_cancel_left' local.le_add local.sum_minus_left)    
-    
-end
-  
-text {* We then define an equivalent class as a pre_trace, where
-        in addition to satisfying fzero_sum_zero, and being a left
-        cancellative semigroup, we also require sum_eq_sum_conv. *}
+    by (metis local.add_diff_cancel_left' local.diff_add_cancel_left' local.le_is_fzero_le local.fzero_le_add local.fzero_le_trans)
 
-context fzero_add_zero
-begin
+  lemma least_zero [simp]: "f0(a) \<le> b"
+    by (metis local.add.semigroup_axioms local.add_fzero_right local.add_left_imp_eq local.le_iff_add semigroup.assoc)
+
+  (* TODO: Check this still works in CTA theory *)
+  lemma not_le_minus [simp]:  "\<not> (a \<le> b) \<Longrightarrow> b - a = f0(b)"
+    by (simp add: local.fzero_subtract_def local.le_is_fzero_le local.minus_def)
+      
+  lemma diff_zero [simp]: "a - f0(b) = a"
+    by (metis local.add.semigroup_axioms local.add_fzero_right local.diff_add_cancel_left' local.fzero_idem local.least_zero semigroup.assoc)
+       
+  lemma diff_cancel [simp]: "a - a = f0(a)"
+    by (metis local.add_diff_cancel_left' local.add_fzero_right local.diff_zero)
+     
+  lemma zero_le_minus_imp_le: "\<lbrakk> b \<le> a; f0(b) < a - b \<rbrakk> \<Longrightarrow> b < a"
+    using local.less_iff local.minus_cancel_le by fastforce
   
-lemma monoid_le_least_zero: "fzero a \<le>\<^sub>d a"
-  by (metis local.add_fzero_left local.monoid_le_add)
+  lemma le_imp_zero_le_minus: "\<lbrakk> b \<le> a; b < a \<rbrakk> \<Longrightarrow> f0(b) < a - b"
+    by (metis local.add_fzero_right local.add_left_strict_mono local.diff_add_cancel_left')
  
-lemma monoid_le_refl: "a \<le>\<^sub>d a"
-  apply (simp add: local.fzero_le_def)
-  by (metis local.add_fzero_right)
+  lemma le_iff_zero_leq_minus: "\<lbrakk> b \<le> a \<rbrakk> \<Longrightarrow> b < a \<longleftrightarrow> f0(b) < a - b"
+    using zero_le_minus_imp_le le_imp_zero_le_minus by blast
+      
+  lemma le_and_minus_is_zero_imp_eq: "\<lbrakk> b < a \<and> a - b = f0(b)\<rbrakk> \<Longrightarrow> b = a"
+    using local.less_iff le_imp_zero_le_minus by force
+      
+  lemma minus_zero_eq: "\<lbrakk> b \<le> a; a - b = f0(b) \<rbrakk> \<Longrightarrow> a = b"
+    using local.le_iff_add by auto
+
+  text \<open> Lemmas of CTA traces \<close>
+
+  (* Sadd:unit *)
+  lemma sadd_unit: "a + b = a \<longrightarrow> b = f0(b)"
+    by (metis local.add.semigroup_axioms local.add_fzero_right local.add_left_imp_eq semigroup.assoc)
+  
+  (* SSub:same *)
+  lemma ssub_same: "c \<le> a \<and> c \<le> b \<longrightarrow> a - c = b - c \<longleftrightarrow> a = b"
+    by (metis local.diff_add_cancel_left')
+      
+  (* SSub:subsub *)    
+  lemma ssub_subsub: "c \<le> a \<and> c \<le> b \<and> b \<le> a \<longrightarrow>(a - c) - (b - c) = a - b"
+    by (metis local.diff_add_cancel_left' local.sum_minus_right)
 
 end
+
+text \<open> Following the approach in Trace_Algebra we define a @{term pre_trace} class,
+       where in addition to satisfying @{term fzero_sum_zero}, and being a left cancellative
+       semigroup, also requires @{term sum_eq_sum_conv}. \<close>
   
-class fzero_pre_trace = semigroup_add_left_cancel + fzero_sum_zero +
+class fzero_pre_trace = semigroup_add_left_cancel_minus_ord  +
   assumes
   sum_eq_sum_conv: "(a + b) = (c + d) \<Longrightarrow> \<exists> e . a = c + e \<and> e + b = d \<or> a + e = c \<and> b = e + d"
 begin
-  
-  (* still unsure whether this should be moved into another class *)
 
-end
+  text {* The set subtraces of a common trace $c$ is totally ordered *} 
+
+  lemma le_common_total: "\<lbrakk> a \<le> c; b \<le> c \<rbrakk> \<Longrightarrow> a \<le> b \<or> b \<le> a"
+    by (metis diff_add_cancel_left' le_add local.sum_eq_sum_conv)
   
+  lemma le_sum_cases: "a \<le> b + c \<Longrightarrow> a \<le> b \<or> b \<le> a"
+    by (simp add: le_common_total)
+            
+  lemma le_sum_cases':
+    "a \<le> b + c \<Longrightarrow> a \<le> b \<or> b \<le> a \<and> a - b \<le> c"
+    apply auto
+    using local.le_sum_cases apply auto[1]
+    by (metis local.add_le_imp_le_left local.diff_add_cancel_left' local.le_sum_cases)
+    
+  lemma le_sum_iff: "a \<le> b + c \<longleftrightarrow> a \<le> b \<or> b \<le> a \<and> a - b \<le> c"
+    by (metis local.add_le_imp_le_left local.add_left_mono local.diff_add_cancel_left' local.le_is_fzero_le local.le_sum_cases local.fzero_le_add local.fzero_le_trans)
+   
+end
+
 instance fzero_pre_trace \<subseteq> semigroup_add_fzero
   by intro_classes  
  
@@ -458,8 +538,8 @@ text {* As stated earlier, there is no antisymmetry unless fzero
         is a constant. *}  
   
 lemma fzero_monoid_le_antisym :
-  fixes a :: "'a::{fzero_is_0,fzero_pre_trace}"
-  assumes "a \<le>\<^sub>d b" "b \<le>\<^sub>d a"
+  fixes a :: "'a::{fzero_is_0,semigroup_add_left_cancel_minus_ord,fzero_sum_zero}"
+  assumes "a \<le>us b" "b \<le>us a"
   shows "a = b"
 proof -
   obtain a' where a': "b = a + a'"
@@ -469,184 +549,177 @@ proof -
     using assms(2) fzero_le_def by auto
 
   have "b' = (b' + a' + b')"
-    by (metis a' add.semigroup_axioms b' left_cancel_semigroup_class.add_left_imp_eq semigroup.assoc)
-
-  hence "fzero b' + fzero b' + b' = (b' + a' + b')"
+    by (metis a' add.assoc b' semigroup_add_left_cancel_class.add_left_imp_eq)
+    
+  hence "f0(b') + f0(b') + b' = (b' + a' + b')"
     by (metis add.semigroup_axioms add_fzero_left semigroup.assoc)
       
-  hence "fzero b' + fzero b' = b' + a'"
-    by (metis (no_types, lifting) add.semigroup_axioms add_fzero_right fzero_is_0 left_cancel_semigroup_class.add_left_imp_eq semigroup.assoc)
+  hence "f0(b') + f0(b') = b' + a'"
+    by (metis (no_types, lifting) add.assoc fzero_is_0 fzero_sum sadd_unit)
       
-  hence "b' + a' = fzero b'"
+  hence "b' + a' = f0(b')"
     by (metis add_fzero_right fzero_is_0)
       
-  hence "a' = fzero a'" "b' = fzero b'"
-    using fzero_sum apply blast
+  hence "a' = f0(a')" "b' = f0(b')"
+    using fzero_sum 
     using \<open>b' + a' = fzero b'\<close> fzero_sum_left by auto
 
   with a' b' show ?thesis
     by (metis add_fzero_right fzero_is_0)
 
 qed
-  
-text {* We then define the trace algebra using fzero. We reprove
-        properties of the monoid-based trace algebra. *}  
 
-class fzero_trace = fzero_pre_trace + semigroup_add_left_cancel_minus_ord
+text \<open> We finally define the extended trace algebra that uses @{term f\<^sub>0}. \<close>
+
+class fzero_trace = fzero_pre_trace + semigroup_add_left_cancel_minus_ord + fzero_sum_zero
 begin
-  
-  lemma least_zero [simp]: 
-     "fzero a \<le> b"
-     by (metis local.add.semigroup_axioms local.add_fzero_right local.add_left_imp_eq local.le_iff_add semigroup.assoc)
-
-  (* TODO: maybe this result can still be established.. but
-           I don't think it is needed.
-
-  lemma not_le_minus [simp]:  "\<not> (a \<le> b) \<Longrightarrow> b - a = fzero b" *)
-      
-  lemma diff_zero [simp]: "a - fzero b = a"
-    by (metis add_assoc local.add_diff_cancel_left local.add_fzero_right)
-       
-  lemma diff_cancel [simp]: "a - a = fzero a"
-    by (metis local.add_fzero_right local.add_diff_cancel_left)
-      
-  lemma zero_le_minus_imp_le: "\<lbrakk> b \<le> a; fzero b < a - b \<rbrakk> \<Longrightarrow> b < a"
-    by (smt local.add.semigroup_axioms local.add_monoid_diff_cancel_left local.le_iff_add local.less_iff local.minus_def semigroup.assoc)
-
-  lemma le_imp_zero_le_minus: "\<lbrakk> b \<le> a; b < a \<rbrakk> \<Longrightarrow> fzero b < a - b"
-    by (metis local.add_fzero_right local.add_diff_cancel_left local.add_le_imp_le_left local.add_left_mono local.le_iff_add local.less_iff)
- 
-  lemma le_iff_zero_leq_minus: "\<lbrakk> b \<le> a \<rbrakk> \<Longrightarrow> b < a \<longleftrightarrow> fzero b < a - b"
-    using zero_le_minus_imp_le le_imp_zero_le_minus by blast
-      
-  lemma le_and_minus_is_zero_imp_eq: "\<lbrakk> b < a \<and> a - b = fzero b\<rbrakk> \<Longrightarrow> b = a"
-    using local.less_iff le_imp_zero_le_minus by force
-      
-  lemma minus_zero_eq: "\<lbrakk> b \<le> a; a - b = fzero b \<rbrakk> \<Longrightarrow> a = b"
-    using local.le_iff_add by auto
-  
+  -- \<open> The following lemma requires fzero_sum_zero. \<close>
   lemma neq_zero_impl_greater:
-    "x \<noteq> fzero x \<Longrightarrow> fzero x < x"
+    "x \<noteq> f0(x) \<Longrightarrow> f0(x) < x"
     by (metis least_zero local.add_fzero_left local.diff_cancel local.fzero_sum_right local.less_iff sum_minus_left)
-
-  text {* The set subtraces of a common trace $c$ is totally ordered *} 
-  lemma le_common_total: "\<lbrakk> a \<le> c; b \<le> c \<rbrakk> \<Longrightarrow> a \<le> b \<or> b \<le> a"
-    by (metis diff_add_cancel_left' le_add local.sum_eq_sum_conv)
-  
-  lemma le_sum_cases: "a \<le> b + c \<Longrightarrow> a \<le> b \<or> b \<le> a"
-    by (simp add: le_common_total)
-            
-  lemma le_sum_cases':
-    "a \<le> b + c \<Longrightarrow> a \<le> b \<or> b \<le> a \<and> a - b \<le> c"
-    by (auto, metis le_sum_cases, metis minus_def le_is_fzero_le add_monoid_diff_cancel_left fzero_le_def sum_eq_sum_conv)
-
-  lemma le_sum_iff: "a \<le> b + c \<longleftrightarrow> a \<le> b \<or> b \<le> a \<and> a - b \<le> c"
-    by (metis le_sum_cases' add_monoid_diff_cancel_left le_is_fzero_le minus_def monoid_le_add_left_mono fzero_le_def monoid_le_trans)
-
-  (* under what circumstances is - associative? *)
 end
   
 text {* This algebra forms a preorder. It turns out this is
         sufficient for the theories on reactive processes. *}  
   
 instance fzero_trace \<subseteq> preorder
-  apply (intro_classes)
-  apply (simp add: less_iff)
-  apply (simp add: fzero_add_zero_class.monoid_le_refl le_is_fzero_le)
-  using le_is_fzero_le 
-  by (metis semigroup_add_class.monoid_le_trans)
-
-instantiation list :: (type) fzero_is_0
-begin
-  definition fzero_list :: "'a list \<Rightarrow> 'a list" where "fzero_list a = []"
-
-  instance by (intro_classes, simp add:fzero_list_def zero_list_def)
-end
-    
-instantiation list :: (type) fzero_add_zero
-begin
+  by (intro_classes)
  
-  instance by (intro_classes, simp_all add:fzero_list_def plus_list_def)
-end
-  
-lemma fzero_le_list:
-  "(xs :: 'a list) \<le>\<^sub>d ys \<longleftrightarrow> xs \<le> ys"
-  apply (simp add: fzero_le_def plus_list_def)
-  using Prefix_Order.prefixE Prefix_Order.prefixI apply blast
-  done
-    
-lemma fzero_subtract_list:
-  "(xs :: 'a list) -\<^sub>d ys = xs - ys"
-  proof (cases "ys \<le> xs")
-    case True
-    then show ?thesis 
-      apply (auto simp add: fzero_subtract_def fzero_le_list minus_list_def less_eq_list_def)
-      apply (rule the_equality)
-      by (simp_all add: fzero_list_def plus_list_def prefix_drop)
-  next
-    case False
-    then have "xs -\<^sub>d ys = (SOME c. \<forall>d. c \<le>\<^sub>d d)"
-      using fzero_le_list
-      by (metis fzero_subtract_def)
-    also have "... = []"
-      apply (rule some_equality)
-      apply (auto simp add:fzero_le_list)
-      using Prefix_Order.prefix_Nil by blast
-    finally show ?thesis
-      by (simp add: False zero_list_def)
-  qed
-    
-instance list :: (type) fzero_trace
-  apply intro_classes
-  apply (simp_all add:fzero_list_def plus_list_def)
-  apply (simp add: append_eq_append_conv2)
-  using Prefix_Order.prefixE Prefix_Order.prefixI
-  apply (simp add: fzero_le_list)
-  apply (simp add: less_le_not_le)
-  by (simp add: fzero_subtract_list)
-
-instantiation nat :: fzero_is_0
-begin
-  
-  definition fzero_nat :: "nat \<Rightarrow> nat" where "fzero_nat a = 0"
- 
-  instance
-    by (intro_classes, auto simp add:fzero_nat_def)
-end
-  
-lemma fzero_le_nat:
-  "(x :: nat) \<le>\<^sub>d y \<longleftrightarrow> x \<le> y"
-  by (simp add: fzero_le_def trace_class.le_iff_add)
-  
-lemma fzero_subtract_nat:
-  "(x :: nat) -\<^sub>d y = x - y"
-  by (auto simp add:fzero_subtract_def fzero_le_nat) 
-    
-instance nat :: fzero_trace
-  apply intro_classes
-  apply (simp_all add: fzero_nat_def)
-  apply (simp add: pre_trace_class.sum_eq_sum_conv)
-  apply (simp add: fzero_le_def trace_class.le_iff_add)
-  apply (simp add: trace_class.less_iff)
-  by (simp add:fzero_subtract_nat)
-    
 (* the following are properties satisfied by left/right restriction semigroups,
    but the fzero_trace class does not satisfy all of them. I do not think that
-   properties related to commutativity are ever satisfied in the general case. *)    
+   properties related to commutativity are ever satisfied in the general case. *)
     
 lemma fzero_restrict0:
   fixes a :: "'a::fzero_trace"
-  shows "fzero(fzero(a) + b) = fzero(a) + fzero b"
-  by (metis add_diff_cancel_left fzero_trace_class.diff_zero)
-    
+  shows "f0(f0(a) + b) = f0(a) + f0(b)"
+  by (metis add.assoc add_fzero_diff_cancel_left add_fzero_right)
+  
 lemma fzero_restrict1:
   fixes a :: "'a::fzero_trace"
-  shows "fzero(a) + b = b + fzero(a + b)"
-  by (metis (no_types, lifting) add_fzero_right add_diff_cancel_left le_add sum_minus_left)
-
+  shows "f0(a) + b = b + f0(a + b)"
+  by (metis add.assoc add_fzero_right semigroup_add_left_cancel_class.add_left_imp_eq)
+  
 lemma fzero_dist_plus:
   fixes a :: "'a::fzero_trace"
-  shows "fzero(a + b) = fzero(a) + fzero(b)"
-  by (metis add.assoc add_fzero_right add_diff_cancel_left)
+  shows "f0(a + b) = f0(a) + f0(b)"
+  by (metis (no_types, lifting) fzero_idem fzero_restrict0 fzero_restrict1 semigroup_add_left_cancel_class.add_left_imp_eq)
+ 
+lemma 
+  fixes a :: "'a::fzero_trace"
+  shows "f0(a + b) = f0(b)"
+  by (metis add.assoc add_fzero_right semigroup_add_left_cancel_class.add_left_imp_eq)
     
+lemma 
+  fixes x :: "'a::fzero_trace"
+  shows "(x + f0(x)) = x"
+  by simp
+    
+lemma    
+  fixes x :: "'a::fzero_trace"
+    and y :: "'a::fzero_trace"
+  shows "f0(x + y) = f0(f0(x)+y)"
+  by (simp add: fzero_dist_plus)
+    
+lemma    
+  fixes x :: "'a::fzero_trace"
+    and y :: "'a::fzero_trace"
+  shows "f0(f0(x) + f0(y)) = f0(y)+f0(x)+f0(y)"  
+    by (metis (mono_tags, lifting) add.assoc fzero_dist_plus fzero_idem fzero_restrict1)
+  
+lemma    
+  fixes x :: "'a::fzero_trace"
+    and y :: "'a::fzero_trace"
+  shows "f0(x) + f0(x) = f0(x)"
+  by (metis add_fzero_right fzero_idem)
+    
+class fzero_is_0_sum_zero = fzero_is_0 + fzero_sum_zero
+
+instance fzero_is_0_sum_zero \<subseteq> monoid_sum_0
+  apply intro_classes
+  apply (metis add_fzero_left fzero_is_0)
+  apply (metis add_fzero_right fzero_is_0)
+  by (metis fzero_is_0 fzero_sum)
+
+text \<open> A semigroup trace with a fixed zero (@{term fzero_is_0}) 
+       is a monoid. \<close>
+
+class fzero_trace_0 = fzero_trace + fzero_is_0
+
+instance fzero_trace_0 \<subseteq> monoid_add
+proof
+  fix a :: "'a::fzero_trace_0"
+  show add_fzero_left: 
+    "0 + a = a"
+    by (metis add_fzero_right fzero_is_0 fzero_restrict1)
+  show add_zero_right: 
+    "a + 0 = a"
+    by (metis add_fzero_right fzero_is_0)
+qed
+
+text \<open> A semigroup trace with a fixed zero (@{term fzero_is_0}) 
+       is a monoid trace. \<close>
+
+instance fzero_trace_0 \<subseteq> trace 
+proof
+  fix a b c d :: "'a::fzero_trace_0"
+  show left_cancellative: 
+    "a + b = a + c \<Longrightarrow> b = c"
+    using semigroup_add_left_cancel_class.add_left_imp_eq by blast
+  show sum_left_zero:
+    "a + b = 0 \<Longrightarrow> a = 0"
+    by (metis add.right_neutral add_fzero_right fzero_sum_left semigroup_add_left_cancel_class.add_left_imp_eq)
+  show sum_eq_conv:
+    "a + b = c + d \<Longrightarrow> \<exists>e. a = c + e \<and> e + b = d \<or> a + e = c \<and> b = e + d"
+    by (simp add: fzero_pre_trace_class.sum_eq_sum_conv)
+  show monoid_le:
+    "(a \<le> b) = (a \<le>\<^sub>m b)"
+    by (simp add: monoid_le_def semigroup_add_left_cancel_minus_ord_class.le_iff_add)
+  show less:
+    "(a < b) = (a \<le> b \<and> \<not> b \<le> a)"
+    by (simp add: fzero_add_fzero_ord_class.less_iff)
+  show minus:
+    "a - b = a -\<^sub>m b"
+    by (metis fzero_add_fzero_ord_minus_class.minus_def fzero_is_0 fzero_subtract_def le_is_fzero_le monoid_le_def monoid_subtract_def semigroup_add_left_cancel_minus_ord_class.le_iff_add)
+qed
+
+text \<open> Similarly, a trace which has a fixed @{term f\<^sub>0} is a semigroup satisfying the 
+       mirror properties of a monoid. \<close>
+
+class trace_fzero_0 = trace + fzero_is_0
+
+instance trace_fzero_0 \<subseteq> fzero_add_zero
+proof
+  fix a b :: "'a::trace_fzero_0"
+  show "f0(f0(a)) = f0(a)"
+    by (simp add: fzero_is_0)
+  show "f0(b) + a = a"
+    by (simp add: fzero_is_0)
+  show "a + f0(a) = a"
+    by (simp add: fzero_is_0)
+qed
+
+text \<open> Hence such a trace is also a semigroup trace. \<close>
+
+instance trace_fzero_0 \<subseteq> fzero_trace
+proof
+  fix a b c d :: "'a::trace_fzero_0"
+  show "(a \<le> b) = (a \<le>us b)"
+    by (simp add: fzero_le_def trace_class.le_iff_add)
+  show "(a < b) = (a \<le> b \<and> \<not> b \<le> a)"
+    by (simp add: trace_class.less_iff)
+  show "a - b = a -us b"
+    by (metis fzero_is_0 fzero_le_def fzero_subtract_def le_is_monoid_le monoid_subtract_def trace_class.le_iff_add trace_class.minus_def)
+  show "a + b = a + c \<Longrightarrow> b = c"
+    by (metis left_cancel_semigroup_class.add_left_imp_eq)
+  show "a + b = c + d \<Longrightarrow> \<exists>e. a = c + e \<and> e + b = d \<or> a + e = c \<and> b = e + d"
+    by (simp add: pre_trace_class.sum_eq_sum_conv)
+  show "a + b = f0(b) \<Longrightarrow> b = f0(b)"
+    by (simp add: fzero_is_0 zero_sum_right)
+qed
+
+text \<open> Therefore, a semigroup trace with a fixed @{term f\<^sub>0} is exactly the same as the
+       monoid trace. This is convenient as any type instantiated with the class @{class trace}
+       can also be instantiated with the class @{class fzero_trace} by defining an appropriate
+       @{term f\<^sub>0}. \<close>
+  
 end
